Ring structure made abstract; head and tail are now pointers. File is type checked

src/samples/Struct.fst
@@ -1,4 +1,4 @@
-module Ring
+module Struct
 
 module B = LowStar.Buffer
 module HS = FStar.HyperStack
@@ -47,37 +47,13 @@ let well_formed_rb (#a:eqtype) (h:HS.mem) (r:ringstruct a): GTot bool
 //  B.length r.tailptr = 1
 
 
+
 let incr_ht_spec (ht:UInt32.t) (rsize:UInt32.t{ UInt32.lt ht rsize}) : GTot  (l:UInt32.t {UInt32.lt l rsize})
   // increment by 1 and check if the buffer is full
   // if so, reset it
  = let ht' = UInt32.add ht 1ul in
   if UInt32.eq ht' rsize then 0ul
   else ht'
-
-let is_rb_full_spec (#a:eqtype) (h:HS.mem) (r:ringstruct a {well_formed_rb h r}): GTot bool
-  = 
-//  let rsize = r.rsize in
-  let head =  B.get h r.headptr 0 in
-  let tail = B.get h  r.tailptr 0 in
-  let rsize = r.rsize in
-  let head' = incr_ht_spec head rsize in  
-  head' = tail
-
-let is_rb_empty_spec (#a:eqtype) (h:HS.mem) (r:ringstruct a): GTot bool
-  = 
-//  let rsize = r.rsize in
-  let head =  B.get h r.headptr 0 in
-  let tail = B.get h  r.tailptr 0 in
-   UInt32.eq head tail
-
-
-
-
-let get_head_spec (#a:eqtype) (h:HS.mem) (r:ringstruct a {well_formed_rb h r}): GTot (r':UInt32.t {UInt32.lt r' r.rsize})
-= B.get h r.headptr 0
-
-let get_tail_spec (#a:eqtype) (h:HS.mem) (r:ringstruct a {well_formed_rb h r}): GTot (r':UInt32.t {UInt32.lt r' r.rsize})
-= B.get h r.tailptr 0
 
 let incr_head_spec (#a:eqtype) (h:HS.mem) (r:ringstruct a {well_formed_rb h r}): GTot (r':UInt32.t {UInt32.lt r' r.rsize})
  = let head = B.get h r.headptr 0 in
@@ -116,76 +92,43 @@ let incr_ht (ht:UInt32.t) (rsize:UInt32.t{UInt32.lt ht rsize}) : Tot  (i:UInt32.
  * pushed into the head position. If not, buffer remains the same.
  * The post-condition also says that the invariants are preserved, and that the buffer is live.
  *)
-let push (#a:eqtype) (r: ringstruct a) (v: a) : ST unit
+let push (#a:eqtype) (r: ringstruct a) (v: a) : ST bool
   (requires fun h -> live_rb h r
                   /\  well_formed_rb h r
-                  /\ not (is_rb_full_spec h r)
                    )
-  (ensures fun h0 _ h1 -> 
+  (ensures fun h0 s h1 -> 
                     live_rb h1 r 
-                    /\ modifies (loc_union (loc_buffer r.rbuf)  (loc_buffer r.headptr)) h0 h1
-//                    /\ (s == false ==>  as_seq h1 r.rbuf == as_seq h0 r.rbuf)
-//                    /\ (s == false ==>  modifies loc_none h0 h1)
+                    /\  modifies (loc_union (loc_buffer r.rbuf)  (loc_buffer r.headptr)) h0 h1
+                    /\ (s == false ==>  as_seq h1 r.rbuf == as_seq h0 r.rbuf)
+                    /\ (s == false ==>  modifies loc_none h0 h1)
                     /\ tail_unmodified_spec h0 h1 r r 
                     /\ well_formed_rb h1 r
-//                    /\ (s = true ==>  as_seq h1 r.rbuf == Seq.upd (as_seq h0 r.rbuf) (UInt32.v (get_head_spec h0 r)) v)
-//                    /\ (s = true) ==>  (get_head_spec h1 r == incr_head_spec h0 r)
-                      /\ as_seq h1 r.rbuf == Seq.upd (as_seq h0 r.rbuf) (UInt32.v (get_head_spec h0 r)) v
-                      /\  get_head_spec h1 r == incr_head_spec h0 r
-                      /\ not (is_rb_empty_spec h1 r)
+                    /\ (s == true ==>  as_seq h1 r.rbuf == Seq.upd (as_seq h0 r.rbuf) (UInt32.v (incr_head_spec h0 r)) v)
                     )
   =
-(* 
+  let rsize = r.rsize in
+  let head =  !* r.headptr in
   let tail = !* r.tailptr in
   let b = is_rb_full rsize head tail in
   if (not b) then
- *)   // update the buffer at head and then
-    // increment the head
-  let rsize = r.rsize in
-  let head =  !* r.headptr in
-  let _ =  r.headptr *= (incr_ht head rsize) in
-  B.upd r.rbuf head v
-     
-noeq
-type option 'a =
- | Error : option 'a
- | Value : v:'a -> option 'a
- 
-(* pop:  pop off the element at tail
- * The pre-condition checks that the invariants of the ringbuffer hold while
- * the post-condition says that the element read from the ringbuffer is same as the 
- * one read from the same index in the sequence formed from buffer. When the ringbuffer is full
- * tail is not modified other tail is modified.
- * The post-condition also says that the invariants are preserved
- *)
-let pop (#a:eqtype) (r: ringstruct a) : ST a 
-  (requires fun h0 -> live_rb h0 r 
-                     /\ well_formed_rb h0 r
-                     /\ not (is_rb_empty_spec h0 r)
-                    )
-  (ensures fun h0 v h1 -> live_rb h1 r
-                   /\ well_formed_rb h1 r
-                   /\ modifies (loc_buffer r.tailptr) h0 h1
-                   /\ as_seq h1 r.rbuf == as_seq h0 r.rbuf
-                   /\ head_unmodified_spec h0 h1 r r 
-                   /\ (v == Seq.index (as_seq h1 r.rbuf) (UInt32.v (get_tail_spec h0 r)))
-                   /\ (get_tail_spec h1 r == incr_tail_spec h0 r)
-  )
-  = 
-  let rsize = r.rsize in
-  let head =  !* r.headptr in
-  let tail = !* r.tailptr in
-  let b = is_rb_empty rsize head tail in
-  if (not b) then
-    // First deref the buffer and then increment the tail
-    let v = B.index r.rbuf tail  in
-    let _ = r.tailptr *=  incr_ht tail rsize in
-    v
-  
+    let head' = incr_ht head rsize  in
+    // increment the head and then update the buffer at head
+    r.headptr *= head';
+    B.upd r.rbuf head' v;
+    let h' = HST.get () in
+    assert( loc_disjoint (loc_buffer r.rbuf) (loc_buffer r.headptr)
+      /\ loc_disjoint (loc_buffer r.rbuf) (loc_buffer r.tailptr)
+      /\ loc_disjoint (loc_buffer r.headptr) (loc_buffer r.tailptr));
+    true
+  // buffer not updated  
+  else  
+    let h' = HST.get () in
+    assert(live_rb h' r);
+    false
 
 
-// The way the fullness of ringbuffer is checked requires that the minimum size is 2
-let init (#a:eqtype) (i: a) (s:UInt32.t {UInt32.gt s 1ul}) (hid: HS.rid) : ST (ringstruct a)
+
+let init (#a:eqtype) (i: a) (s:UInt32.t {UInt32.gt s 0ul}) (hid: HS.rid) : ST (ringstruct a)
 (requires fun h -> true
 /\ is_eternal_region hid)
 (ensures fun h0 res h1 -> B.modifies B.loc_none h0 h1
@@ -194,10 +137,6 @@ let init (#a:eqtype) (i: a) (s:UInt32.t {UInt32.gt s 1ul}) (hid: HS.rid) : ST (r
 /\ B.fresh_loc (loc_buffer res.tailptr) h0 h1 
 /\ well_formed_rb h1 res
 /\ live_rb h1 res
-/\ B.length res.rbuf == UInt32.v s
-/\ (is_rb_empty_spec h1 res)
-/\ not (is_rb_full_spec h1 res)
-/\ res.rsize = s
 )
  =
   {rbuf = B.malloc hid i s; headptr =  B.malloc hid 0ul 1ul; tailptr =  B.malloc hid 0ul 1ul; rsize=s}
@@ -207,38 +146,19 @@ let init (#a:eqtype) (i: a) (s:UInt32.t {UInt32.gt s 1ul}) (hid: HS.rid) : ST (r
 (* A simple program that pushes and pops an element from ring buffer
  * The specification says that when operations are successful, the popped element 
  * should be equal to the pushed element. Else, we don't care.
+ * For simplicity, 16l is hardcoded.
  *)
-let test_ringbuffer (): ST UInt8.t
-(requires fun h0 -> true)
-(requires fun h0 v h1 -> v == 4uy)
-= 
-let rlen = 32ul in
+let test_ringbuffer (): ST unit
+     (requires fun h0 -> true)
+     (ensures fun h0 r h1 -> true) 
+     =
+  let rlen = 32ul in
   let rinit = 1uy in
   //ringbuffer is located in host memory region but is disjoint from the host_memory
   let rb = init rinit rlen HS.root in
-//  let h' = HST.get () in
-//  assert(live_rb h' rb);
-//  assert(not (is_rb_full_spec h' rb));
-  let _ = push rb 3uy in
-//  let h'' = HST.get () in
-//  assert(B.live h'' rb.headptr);
-//  assert(not (is_rb_empty_spec h'' rb));
- // let hd = !* (rb.headptr) in
-//  assert(B.live h'' rb.headptr);
-//  assert((B.get h'' rb.headptr 0) = (incr_head_spec h' rb));
-//  assert(hd = (incr_head_spec h' rb));
-  let _ = pop rb in  
-  let _ = push rb 4uy in
-  let v = pop rb in
-  v
-
-   
-(*
-let main () : ST Int32.t
-  (requires fun h0 -> true)
-  (ensures fun h0 r h1 -> true)
-  = 
-  let _ = test_ringbuffer () in
-  0l
-
-*)
+  let status = push rb 2uy in
+  let h' = HST.get () in
+  assert(
+  //B.live h' rb.rbuf);
+   B.live h' rb.headptr)
+ // B.live h' rb.tailptr);
